examples/CCS/ExampleScript.sml
@@ -204,64 +204,23 @@ in
                                 (combine (["ex_A1", "ex_A2", "ex_A3"], nodes))
 end;
 
-val (WB_rules, WB_coind, WB_cases) = Hol_coreln `
-    (!(P :('a, 'b) CCS) (Q :('a, 'b) CCS).
-       (!l.
-         (!P'. TRANS P (label l) P' ==>
-               (?Q'. WEAK_TRANS Q (label l) Q' /\ WB P' Q')) /\
-         (!Q'. TRANS Q (label l) Q' ==>
-               (?P'. WEAK_TRANS P (label l) P' /\ WB P' Q'))) /\
-       (!P'. TRANS P tau P' ==> (?Q'. EPS Q Q' /\ WB P' Q')) /\
-       (!Q'. TRANS Q tau Q' ==> (?P'. EPS P P' /\ WB P' Q'))
-     ==> WB P Q)`;
+(* Examples used in Section 5 of I&C paper *)
+Theorem WG_example1 :
+    WG (\t. prefix a t + prefix b t + prefix c (var Y))
+Proof
+    HO_MATCH_MP_TAC WG4
+ >> Reverse CONJ_TAC >- REWRITE_TAC [WG2]
+ >> HO_MATCH_MP_TAC WG4
+ >> REWRITE_TAC [WG1]
+QED
 
-(* SOS rules with changed variable names *)
-val PREFIX' = store_thm (
-   "PREFIX'", ``!P u. TRANS (prefix u P) u P``,
-    PROVE_TAC [PREFIX]);
-
-val SUM1' = store_thm (
-   "SUM1'",
-  ``!P u P' Q. TRANS P u P' ==> TRANS (sum P Q) u P'``,
-    PROVE_TAC [SUM1]);
-
-val SUM2' = store_thm (
-   "SUM2'",
-  ``!P u P' Q. TRANS P u P' ==> TRANS (sum Q P) u P'``,
-    PROVE_TAC [SUM2]);
-
-val PAR1' = store_thm (
-   "PAR1'",
-  ``!P u P' Q. TRANS P u P' ==> TRANS (par P Q) u (par P' Q)``,
-    PROVE_TAC [PAR1]);
-
-val PAR2' = store_thm (
-   "PAR2'",
-  ``!P u P' Q. TRANS P u P' ==> TRANS (par Q P) u (par Q P')``,
-    PROVE_TAC [PAR2]);
-
-val PAR3' = store_thm (
-   "PAR3'",
-  ``!P l P' Q P2. TRANS P (label l) P' /\ TRANS Q (label (COMPL l)) Q'
-              ==> TRANS (par P Q) tau (par P' Q')``,
-    PROVE_TAC [PAR3]);
-
-val RESTR' = store_thm (
-   "RESTR'",
-  ``!P u Q l L. TRANS P u Q /\ ((u = tau) \/
-                                ((u = label l) /\ l NOTIN L /\ (COMPL l) NOTIN L))
-            ==> TRANS (restr L P) u (restr L Q)``,
-    PROVE_TAC [RESTR]);
-
-val RELABELING' = store_thm (
-   "RELABELING'",
-  ``!P u Q rf. TRANS P u Q ==> TRANS (relab P rf) (relabel rf u) (relab Q rf)``,
-    PROVE_TAC [RELABELING]);
-
-val REC' = store_thm (
-   "REC'",
-  ``!P u A P'. TRANS (CCS_Subst P (rec A P) A) u P' ==> TRANS (rec A P) u P'``,
-    PROVE_TAC [REC]);
+Theorem WG_example2 :
+    WG (\t. prefix a (var X) + prefix b (var X) + prefix c t)
+Proof
+    HO_MATCH_MP_TAC WG4
+ >> Reverse CONJ_TAC >- REWRITE_TAC [WG1]
+ >> REWRITE_TAC [WG2]
+QED
 
 val _ = export_theory ();
 val _ = html_theory "Example";
